theories/Lowering/ParallelMove.v
@@ -2,7 +2,7 @@ Require Import CSet Le.
 
 Require Import Plus Util AllInRel InRel Map MapUpdate MapDefined.
 Require Import Val Var Envs IL NoParams Annotation SimI Fresh.
-Require Import Liveness.Liveness Status InfinitePartition AppExpFree.
+Require Import Liveness.Liveness Status InfiniteSubset InfinitePartition AppExpFree.
 Require compcert.lib.Parmov.
 
 Set Implicit Arguments.
@@ -46,6 +46,51 @@ Proof.
   cset_tac.
 Qed.
 
+
+Lemma combine_get A B (Z:list A) (Y:list B) n x y
+  : get Z n x -> get Y n y -> get (combine Z Y) n (x,y).
+Proof.
+  intros GET1 GET2.
+  general induction GET1; try inv GET2; clear_trivial_eqs; simpl;
+    eauto using get.
+Qed.
+
+Lemma move_no_temp_notin m pmtmp
+  : pmtmp ∉ of_list (fst ⊝ m) ∪ of_list (snd ⊝ m)
+    <-> Parmov.move_no_temp positive (fun _ : positive => pmtmp) m.
+Proof.
+  assert (EqDec:EqDec (positive * positive) eq). {
+    hnf; intros.
+    decide (x === y). left. invc e. rewrite H, H0. reflexivity.
+    right; intro. invc H. eauto.
+  }
+  split; hnf; intros; hnf; intros.
+  - split; hnf; intros.
+    + eapply in_get in H0 as [? ?]; eauto.
+      hnf; intros; subst.
+      cset_tac'. eapply H0.
+      eapply get_in_of_list.
+      eapply map_get_eq; eauto.
+    + eapply in_get in H0 as [? ?]; eauto.
+      hnf; intros; subst.
+      cset_tac'. eapply H1.
+      eapply get_in_of_list.
+      eapply map_get_eq; eauto.
+  - cset_tac'.
+    + edestruct of_list_get_first; eauto; dcr. invc H2.
+      inv_get.
+      exploit (H (fst x1) (snd x1)).
+      eapply get_in; eauto using combine_get; eauto.
+      * rewrite <- pair_eta; eauto.
+      * dcr. eapply H2; eauto. eapply 1%positive.
+    + edestruct of_list_get_first; eauto; dcr. invc H2.
+      inv_get.
+      exploit (H (fst x1) (snd x1)).
+      eapply get_in; eauto using combine_get; eauto.
+      * rewrite <- pair_eta; eauto.
+      * dcr. eapply H4; eauto. eapply 1%positive.
+Qed.
+
 Section ParmovSourceSet.
   Import Parmov.
 
@@ -82,6 +127,15 @@ Section ParmovSourceSet.
     - etransitivity; eauto.
   Qed.
 
+  Lemma dtransitions_dst_set t st st'
+    : dtransitions var t st st' ->
+      st_source_set st' ⊆ st_source_set st.
+  Proof.
+    intros TR.
+    general induction TR; simpl in *; eauto using dtransition_source_set.
+    - etransitivity; eauto.
+  Qed.
+
   Lemma parmove_src_set t mu
     : moves_source_set (parmove var var_dec t mu) ⊆ of_list (fst ⊝ mu).
   Proof.
@@ -100,7 +154,7 @@ Proof.
   firstorder.
 Qed.
 
-Notation "f [ // p ]" := (@Parmov.exec_seq var var_dec _ p f) (at level 29, left associativity).
+Notation "f <||= p" := (@Parmov.exec_seq var var_dec _ p f) (at level 29, left associativity).
 
 Lemma Parmov_update_eq M x y
   : Parmov.update var var_dec (؟ val) x y M = M [x <- y].
@@ -120,7 +174,7 @@ Section GlueCode.
   Lemma list_to_stmt_correct (p:Parmov.moves var) s (M:onv val) K
         (Def:defined_on (moves_source_set p) M)
     : star2 I.step (K, M, list_to_stmt p s) nil
-        (K, M [ // p ], s).
+        (K, M <||= p, s).
   Proof.
     general induction p.
     - firstorder using star2.
@@ -157,16 +211,16 @@ Section GlueCode.
     eapply In_InA; eauto.
   Qed.
 
-  Lemma list_to_stmt_correct' D (m:Parmov.moves var) (M M':onv val) x
+  Lemma parmov_update_with_list D (m:Parmov.moves var) (M:onv val) x
         (ND:NoDupA eq (snd ⊝ m))
-        (NOTIN : Parmov.move_no_temp var (fun _ => x) m)
+        (NOTIN : x ∉ of_list (fst ⊝ m) ∪ of_list (snd ⊝ m))
     : agree_on eq (D \ singleton x)
-               (M[ // Parmov.parmove var var_dec (fun _ => x) m])
+               (M <||= Parmov.parmove var var_dec (fun _ => x) m)
                (M [ snd ⊝ m <-- lookup_list M (fst ⊝ m) ]).
   Proof.
     intros.
     exploit (@Parmov.parmove_correctness var var_dec (fun _ => x) (option val) m).
-    - eauto.
+    - rewrite <- move_no_temp_notin. eauto.
     - eapply NoDup_is_mill; eauto.
     - rewrite <- exec_par_eq.
       hnf; intros.
@@ -184,45 +238,14 @@ Fixpoint onlyVars (Y:args) : params :=
     | (Var x)::Y => x::onlyVars Y
     | _::Y => onlyVars Y
   end.
-(*
-Lemma onlyVars_defined (E:onv val) Y Y' v
-  : onlyVars Y = Y'
-    -> omap (op_eval E) Y = Some v
-    -> forall x, x ∈ of_list Y' -> E x <> None.
+
+Lemma lookup_list_var_map (E:onv val) Y v
+  : omap (op_eval E) (Var ⊝ Y) = Some v
+    -> lookup_list E Y = Some ⊝ v.
 Proof.
   intros. general induction Y; simpl in * |- *; eauto.
-  - inv H; simpl in *. cset_tac; intuition.
-  - destruct a; isabsurd. monadS_inv H. monad_inv H0.
-    simpl in * |- *.
-    cset_tac; congruence.
+  monad_inv H; simpl. f_equal; eauto.
 Qed.
-
-Lemma onlyVars_defined_on (E:onv val) Y Y' v
-  : onlyVars Y = Success Y'
-    -> omap (op_eval E) Y = Some v
-    -> defined_on (of_list Y') E.
-Proof.
-  intros. general induction Y; simpl in * |- *; eauto.
-  - inv H; simpl in *. hnf; cset_tac.
-  - destruct a; isabsurd. monadS_inv H. monad_inv H0.
-    simpl in * |- *.
-    exploit IHY; eauto.
-    hnf; cset_tac.
-Qed.
- *)
-
-Lemma onlyVars_lookup (E:onv val) Y v
-      (AEF:forall (n : nat) (y : op), get Y n y -> isVar y)
-  : omap (op_eval E) Y = Some v
-    -> lookup_list E (onlyVars Y) = List.map Some v.
-Proof.
-  intros. general induction Y; simpl in * |- *; eauto.
-  monad_inv H.
-  exploit AEF as IV; eauto using get. inv IV; eauto; simpl.
-  simpl in *.
-  f_equal; eauto. eapply IHY; eauto using get.
-Qed.
-
 
 Lemma onlyVars_length Y
       (AEF:forall (n : nat) (y : op), get Y n y -> isVar y)
@@ -233,48 +256,63 @@ Proof.
   rewrite IHY; eauto using get.
 Qed.
 
-Lemma onlyVars_eq Y
-      (AEF:forall (n : nat) (y : op), get Y n y -> isVar y)
-  : Y = Var ⊝ onlyVars Y.
+Lemma onlyVars_idem Y
+  : onlyVars (Var ⊝ Y) = Y.
 Proof.
-  general induction Y; simpl; eauto.
-  exploit AEF; eauto using get. inv H; simpl.
-  rewrite <- IHY; eauto using get.
+  general induction Y; simpl; f_equal; eauto.
 Qed.
 
 Hint Resolve onlyVars_length : len.
 
+Definition repl (Z:params) x y := (fun z => if [x === z] then y else z) ⊝ Z.
 
-Fixpoint lower (p:inf_partition var) (DL:〔⦃var⦄ * params〕) s (an:ann (set var))
+Instance pos_lt_computable x y : Computable ((x <= y)%positive).
+Proof.
+  hnf; intros. unfold Pos.le.
+  destruct (x ?= y)%positive.
+  - left; discriminate.
+  - left; discriminate.
+  - right; eauto.
+Qed.
+
+Fixpoint lower (p:inf_partition var) (preg:var) (DL:〔⦃var⦄ * params〕) s (an:ann (set var))
   : stmt :=
   match s, an with
-    | stmtLet x e s, ann1 lv ans => stmtLet x e (lower p DL s ans)
-    | stmtIf x s t, ann2 lv ans ant => stmtIf x (lower p DL s ans) (lower p DL t ant)
+    | stmtLet x e s, ann1 lv ans => stmtLet x e (lower p preg DL s ans)
+    | stmtIf x s t, ann2 lv ans ant => stmtIf x (lower p preg DL s ans) (lower p preg DL t ant)
     | stmtApp l Y, ann0 lv  =>
       let '(lv', Z) := nth_default (∅, nil) DL (counted l) in
       let x := least_fresh_P (part_2 p) (lv' ∪ lv) in
-      let mvs := Parmov.parmove2 var var_dec (fun _ => x) (onlyVars Y) Z in
-      list_to_stmt mvs (stmtApp l nil)
+      let z := least_fresh_P (part_2 p) ({x; lv'} ∪ lv) in
+      let r := least_fresh_P (part_1 p) (lv' \ of_list Z ∪ lv) in
+      if [ (r <= preg)%positive ] then
+        let mvs := Parmov.parmove2 var var_dec (fun _ => x) (onlyVars Y) Z in
+        list_to_stmt mvs (stmtApp l nil)
+      else
+        let r := proj1_sig (InfiniteSubset.inf_subset_least (part_1 p)) in
+        let mvs := Parmov.parmove2 var var_dec (fun _ => x) (repl (onlyVars Y) r z) (repl Z r z) in
+        list_to_stmt ((r,z)::mvs++(z,r)::nil) (stmtApp l nil)
     | stmtReturn x, ann0 lv => stmtReturn x
     | stmtFun F t, annF lv ans ant =>
       let DL' := pair ⊜ (getAnn ⊝ ans) (fst ⊝ F) in
-      let s' := zip (fun Zs a => lower p (DL' ++ DL) (snd Zs) a) F ans in
-      let t' := lower p (DL' ++ DL) t ant in
+      let s' := zip (fun Zs a => lower p preg (DL' ++ DL) (snd Zs) a) F ans in
+      let t' := lower p preg (DL' ++ DL) t ant in
       (stmtFun ((fun s => (nil, s)) ⊝ s') t')
     | _, _ => s
   end.
 
 Inductive approx
-: list (set var) -> list I.block -> list I.block -> ⦃var⦄ -> I.block -> I.block -> Prop :=
-  approxI L L' DL Z s s' lv n p
+  : inf_partition var -> var ->
+    list (set var) -> list I.block -> list I.block -> ⦃var⦄ -> I.block -> I.block -> Prop :=
+  approxI L L' DL Z s s' lv n p preg
   (al:ann (set var))
   (LS:live_sound Imperative (I.block_Z ⊝ L) DL s al)
   (AL:(of_list Z) ⊆ lv)
   (AEF:app_expfree s)
   (ND:NoDupA eq Z)
   (INCL:getAnn al \ of_list Z ⊆ lv)
-  (spm:lower p (zip pair DL (I.block_Z ⊝ L)) s al = s')
-  : approx DL L L' lv (I.blockI Z s n) (I.blockI nil s' n).
+  (spm:lower p preg (zip pair DL (I.block_Z ⊝ L)) s al = s')
+  : approx p preg DL L L' lv (I.blockI Z s n) (I.blockI nil s' n).
 
 
 Lemma omap_var_defined_on Za E vl
@@ -289,81 +327,353 @@ Proof.
     hnf; intros. cset_tac.
 Qed.
 
-Lemma correct p Lv L L' s (E E':onv val) (al: ann (set var))
+Lemma fst_combine A B (L:list A) (L':list B) (Len:❬L❭=❬L'❭)
+  : fst ⊝ combine L L' = L.
+Proof.
+  general induction Len; simpl; f_equal; eauto.
+Qed.
+
+Lemma snd_combine A B (L:list A) (L':list B) (Len:❬L❭=❬L'❭)
+  : snd ⊝ combine L L' = L'.
+Proof.
+  general induction Len; simpl; f_equal; eauto.
+Qed.
+
+Lemma repl_not_in Z x y
+  : x ∉ of_list Z -> repl Z x y = Z.
+Proof.
+  general induction Z; simpl; repeat cases; simpl in *; eauto.
+  - invc COND. cset_tac.
+  - f_equal. eapply IHZ; cset_tac.
+Qed.
+
+Lemma repl_not_in' Z x y x'
+  : x ∉ of_list Z -> x =/= y -> x ∉ of_list (repl Z x' y).
+Proof.
+  general induction Z; simpl; repeat cases; simpl in *; eauto.
+  - invc COND. cset_tac.
+  - exploit (IHZ x y); eauto. cset_tac. cset_tac.
+Qed.
+
+Lemma repl_nodup Z x y
+  : y ∉ of_list Z -> NoDupA eq Z -> NoDupA eq (repl Z x y).
+Proof.
+  intros IN ND.
+  general induction ND; simpl; repeat cases; simpl in *; eauto using NoDupA.
+  - invc COND. econstructor; eauto.
+    + rewrite repl_not_in; cset_tac.
+    + eapply IHND. cset_tac.
+  - econstructor; eauto.
+    + exploit (@repl_not_in' l x y x0); eauto. cset_tac. cset_tac.
+    + eapply IHND; eauto. cset_tac.
+Qed.
+
+Lemma of_list_repl_incl Z x y
+  : of_list (repl Z x y) ⊆ {y; of_list Z}.
+Proof.
+  general induction Z; simpl; repeat cases; eauto.
+  - cset_tac.
+  - rewrite IHZ; cset_tac.
+  - rewrite IHZ; cset_tac.
+Qed.
+
+Lemma repl_get_ne (Z:params) n (x y z:var)
+  : get Z n z -> z =/= x -> get (repl Z x y) n z.
+Proof.
+  intros GET. general induction GET; simpl; repeat cases; eauto using get.
+Qed.
+
+Lemma repl_get_eq (Z:params) n (x y z:var)
+  : get Z n x -> get (repl Z x y) n y.
+Proof.
+  intros GET. general induction GET; simpl; repeat cases; eauto using get.
+Qed.
+
+Lemma repl_get_inv (Z:params) n (x y z:var)
+  : get (repl Z x y) n z -> z =/= y -> get Z n z.
+Proof.
+  intros GET.
+  general induction Z; simpl in *; repeat cases in GET; inv GET; eauto using get.
+Qed.
+
+Lemma parmov_repl_agree lv (E:onv val) (pmtmp reg lstmp:var) (Y Z:params) (Len:❬Y❭=❬Z❭) (NEQ:reg =/= lstmp) (NEQ2:pmtmp =/= lstmp)
+      (NDZ:NoDupA _eq Z) (NOTIN:lstmp ∉ of_list Y ∪ of_list Z) (NOTIN2: pmtmp ∉ of_list Y ∪ of_list Z)
+  : agree_on eq (lv \ {lstmp; singleton pmtmp})
+             (E <||= Parmov.parmove2 positive var_dec (fun _ : positive => pmtmp) Y Z)
+             (E <||=
+                ((reg, lstmp)
+                   :: Parmov.parmove2 positive var_dec (fun _ : positive => pmtmp) (repl Y reg lstmp)
+                   (repl Z reg lstmp) ++ (lstmp, reg) :: nil)).
+Proof.
+  simpl; rewrite Parmov.exec_seq_app; simpl.
+  rewrite !Parmov_update_eq.
+  set (ZR:=repl Z reg lstmp) in *.
+  set (YR:=repl Y reg lstmp) in *.
+  set (PM:=Parmov.parmove2 positive var_dec (fun _ : positive => pmtmp) (repl Y reg lstmp)
+                           (repl Z reg lstmp)) in *.
+  etransitivity. {
+    eapply agree_on_incl.
+    eapply parmov_update_with_list; eauto.
+    + rewrite snd_combine; eauto with len.
+    + rewrite fst_combine, snd_combine; eauto with len.
+    + cset_tac.
+  }
+  symmetry. etransitivity. {
+    eapply agree_on_update_same. reflexivity.
+    eapply agree_on_incl.
+    eapply parmov_update_with_list; eauto.
+    + rewrite snd_combine; eauto with len.
+      eapply repl_nodup; eauto. cset_tac.
+    + rewrite fst_combine, snd_combine; eauto with len.
+      subst ZR YR. rewrite !of_list_repl_incl. cset_tac.
+    + cset_tac.
+  }
+  symmetry.
+  rewrite snd_combine, fst_combine; eauto with len.
+  hnf; intros. lud.
+  - unfold Parmov.parmove2.
+    erewrite parmov_update_with_list; eauto;
+      try rewrite snd_combine; try rewrite fst_combine; eauto with len.
+    + invc H2; clear e.
+      decide (reg ∈ of_list Z).
+      * eapply of_list_get_first in i; dcr. symmetry in H5; invc H5.
+        exploit (@update_with_list_lookup_in_list_first _ _ _ E x Z (lookup_list E Y)); dcr;
+          eauto with len.
+        rewrite H9. rewrite lookup_list_map in H8. inv_get. rewrite <- EQ.
+        exploit repl_get_eq; try eapply H2; eauto.
+        exploit (@update_with_list_lookup_in_list_first _ _ _ (E [lstmp <- E reg]) x ZR (lookup_list (E [lstmp <- E reg]) YR)); dcr;
+          eauto with len.
+        -- intros. intro. invc H6.
+           unfold ZR in H5. unfold repl in H5. inv_get. cases in EQ0.
+           ++ eapply H7. eauto. eauto. eauto.
+           ++ subst.
+             eapply get_in_of_list in H5. cset_tac.
+        -- rewrite H9.
+           rewrite lookup_list_map in H6. subst YR. unfold repl in H6.
+           inv_get. cases in H4.
+           ++ invc COND.
+             rewrite <- H4. lud. cset_tac.
+           ++ unfold repl in H3. inv_get.
+             cases in H3.
+             rewrite <- H4. lud. invc H6.
+             eapply get_in_of_list in H8. exfalso. cset_tac.
+      * rewrite !lookup_set_update_not_in_Z; eauto.
+        lud. cset_tac.
+        subst ZR. rewrite repl_not_in; eauto. cset_tac.
+    + eapply repl_nodup; eauto. cset_tac.
+    + subst ZR YR. rewrite !of_list_repl_incl. cset_tac.
+    + instantiate (1:=singleton lstmp). cset_tac.
+  - rewrite fst_combine, snd_combine; eauto with len.
+    decide (x ∈ of_list Z).
+    + eapply of_list_get_first in i; dcr. symmetry in H5; invc H5.
+      exploit (@update_with_list_lookup_in_list_first _ _ _ E x0 Z (lookup_list E Y)); dcr;
+        eauto with len.
+      rewrite H9.
+      rewrite lookup_list_map in H8. inv_get. rewrite <- EQ.
+      exploit repl_get_ne; try eapply H4; eauto.
+      exploit (@update_with_list_lookup_in_list_first _ _ _ (E [lstmp <- E reg]) x0 ZR (lookup_list (E [lstmp <- E reg]) YR)); dcr;
+        eauto with len.
+      * subst ZR. intros. unfold repl in *. inv_get.
+        repeat cases; eauto. invc COND.
+        intro. invc H5.
+        cset_tac.
+      * subst YR. rewrite lookup_list_map in H10.
+        unfold repl in H5, H10. inv_get.
+        repeat cases; eauto.
+        cases in H6.
+        -- invc COND.
+           rewrite <- H6. lud; eauto.
+        -- rewrite <- H6. lud; eauto. invc H10. clear e.
+           exfalso. clear - H8 NOTIN.
+           eapply get_in_of_list in H8.
+           cset_tac'.
+    + rewrite !lookup_set_update_not_in_Z; eauto.
+      lud. cset_tac.
+      eapply repl_not_in'; eauto. cset_tac.
+Qed.
+
+Local Arguments list_to_stmt : simpl never.
+Local Arguments Parmov.exec_seq : simpl never.
+
+
+Lemma correct (p:inf_partition var) (preg:var) Lv L L' s (E E':onv val) (al: ann (set var))
       (LS:live_sound Imperative (I.block_Z ⊝ L) Lv s al)
       (AEF:app_expfree s)
- (LA:inRel approx Lv L L')
- (EEQ:agree_on eq (getAnn al) E E')
-  : sim bot3 Sim (L,E,s) (L', E', lower p (zip pair Lv (I.block_Z ⊝ L))  s al).
+      (LA:inRel (approx p preg) Lv L L')
+      (EEQ:agree_on eq (getAnn al) E E')
+      (DEF:defined_on (getAnn al) E) (PREG1: part_1 p preg)
+  : sim bot3 Sim (L,E,s) (L', E', lower p preg (zip pair Lv (I.block_Z ⊝ L))  s al).
 Proof.
   revert_all. pcofix pmSim_sim; intros.
   inv LS; inv AEF; simpl in *.
   - invt live_exp_sound.
     + eapply (sim_let_op il_statetype_I);
-        eauto 20 using op_eval_live, agree_on_update_same, agree_on_incl.
-    + eapply (sim_let_call il_statetype_I); eauto 10 using agree_on_update_same, agree_on_incl.
+        eauto 20 using op_eval_live, agree_on_update_same, agree_on_incl,
+        defined_on_update_some, defined_on_incl.
+    + eapply (sim_let_call il_statetype_I);
+        eauto 10 using agree_on_update_same, agree_on_incl,
+        defined_on_update_some, defined_on_incl.
         erewrite <- omap_op_eval_live_agree; eauto. eapply agree_on_sym; eauto.
   - eapply (sim_cond il_statetype_I);
-      eauto 20 using op_eval_live, agree_on_update_same, agree_on_incl.
+      eauto 20 using op_eval_live, agree_on_update_same, agree_on_incl, defined_on_incl.
   - rewrite nth_default_eq. erewrite get_nth; eauto using zip_get; simpl.
     inRel_invs.
     inv_get. simpl in *.
-    case_eq (omap (op_eval E) Y); intros.
-    + exploit onlyVars_length as Len; eauto.
-      exploit (Parmov.srcs_dests_combine _ (onlyVars Y) Z0) as Eq; eauto with len.
-      destruct Eq as [SrcEq DstEq]. unfold Parmov.srcs, Parmov.dests in *.
+    eapply op_eval_var in H5 as [Y' ?]; subst Y.
+    rewrite onlyVars_idem in *. len_simpl.
+    case_eq (omap (op_eval E) (Var ⊝ Y')); intros.
+    + set (reg:=least_fresh_P (part_1 p) (blv \ of_list Z0 ∪ lv)) in *.
+      set (lreg:=InfiniteSubset.inf_subset_least (part_1 p)) in *.
+      set (pmtmp := least_fresh_P (part_2 p) (blv ∪ lv)) in *.
+      set (lstmp := least_fresh_P (part_2 p) ({pmtmp; blv} ∪ lv)) in *.
+      assert (NEQ1:reg =/= lstmp). {
+        subst reg lstmp.
+        intro.
+        eapply (part_disj p (least_fresh_P (part_1 p) (blv \ of_list Z0 ∪ lv))); eauto.
+        eapply least_fresh_P_full_spec.
+        rewrite H5.
+        eapply least_fresh_P_full_spec.
+      }
+      assert (NEQ2: pmtmp =/= lstmp). {
+        subst pmtmp lstmp. intro.
+        eapply (least_fresh_P_full_spec (part_2 p) ({least_fresh_P (part_2 p) (blv ∪ lv); blv} ∪ lv)).
+        rewrite <- H5. clear. cset_tac.
+      }
+      assert (NEQ3:proj1_sig lreg =/= lstmp). {
+        subst lreg lstmp. destr_sig; dcr.
+        intro. invc H7.
+        eapply (part_disj p); eauto.
+        eapply least_fresh_P_full_spec.
+      }
+      assert (pmtmp ∉ of_list Y' ∪ blv). {
+        intro.
+        eapply (least_fresh_P_full_spec (part_2 p) (blv ∪ lv)).
+        eapply Ops.freeVars_live_list in H3.
+        rewrite <- of_list_freeVars_vars in H3. rewrite <- H3 at 2.
+        setoid_rewrite union_comm at 2. eauto.
+      }
+      assert (lstmp ∉ of_list Y' ∪ blv). {
+        intro.
+        eapply (least_fresh_P_full_spec (part_2 p) ({pmtmp; blv} ∪ lv)).
+        eapply Ops.freeVars_live_list in H3.
+        rewrite <- of_list_freeVars_vars in H3. rewrite <- H3 at 2.
+        setoid_rewrite union_comm at 2.
+        setoid_rewrite <- incl_add' at 2. eauto.
+      }
+      unfold Parmov.srcs, Parmov.dests in *.
       exploit omap_op_eval_live_agree; try eassumption.
-      exploit (@list_to_stmt_correct
-                 (Parmov.parmove2 var var_dec (fun _ => least_fresh_P (part_2 p) (blv ∪ lv)) (onlyVars Y) Z0)
-                 (stmtApp l nil) E' L').
-
-      unfold Parmov.parmove2.
-      rewrite parmove_src_set. rewrite SrcEq.
-      rewrite (onlyVars_eq H5) in H6.
-      eapply omap_var_defined_on; eauto.
-      pfold. eapply SimSilent.
-      * eapply plus2O. econstructor; eauto. simpl. reflexivity.
-      * eapply star2_plus2_plus2 with (A:=nil) (B:=nil); eauto.
-        eapply plus2O. econstructor; eauto. reflexivity. reflexivity.
-      * right; eapply pmSim_sim; try eapply LA1; eauto; simpl.
-        -- eapply (inRel_drop LA H4).
-        -- assert (getAnn al ⊆ blv) by eauto with cset.
-           symmetry. etransitivity.
-           eapply agree_on_incl.
-           eapply (@list_to_stmt_correct' (getAnn al)); eauto.
-           ++ rewrite DstEq. eauto.
-           ++ assert (of_list (onlyVars Y) ⊆ lv). {
-               eapply Ops.freeVars_live_list in H3.
-               rewrite <- H3. rewrite (onlyVars_eq H5) at 2.
-               rewrite of_list_freeVars_vars. reflexivity.
-             }
-             hnf; intros ? ? IN.
-             split.
-             eapply in_combine_l in IN.
-             hnf. intros.
-             intro; subst.
-             eapply In_InA in IN.
-             eapply of_list_1 in IN.
-             rewrite H9 in IN. rewrite (incl_right _ lv blv) in IN at 2.
-             eapply least_fresh_P_full_spec in IN; eauto. eauto.
-             eapply in_combine_r in IN.
-             hnf. intros.
-             intro; subst.
-             eapply In_InA in IN.
-             eapply of_list_1 in IN.
-             rewrite AL in IN. rewrite (incl_left _ blv lv) in IN at 2.
-             eapply least_fresh_P_full_spec in IN; eauto. eauto.
-           ++ rewrite disj_minus_eq; eauto.
-             rewrite H8; clear.
-             intro; hnf; intros.
-             eapply (incl_left _ blv lv) in H.
-             eapply (least_fresh_P_full_spec (part_2 p) (blv ∪ lv)).
-             cset_tac.
-           ++ rewrite SrcEq, DstEq.
-             erewrite onlyVars_lookup; eauto.
-             eapply update_with_list_agree; eauto with len.
-             symmetry.
-             eapply agree_on_incl; eauto. eauto with cset.
+      {
+        cases.
+        - exploit (@list_to_stmt_correct
+                     (Parmov.parmove2 positive var_dec (fun _ : positive => pmtmp) Y' Z0)
+                     (stmtApp l nil) E' L'). {
+            unfold Parmov.parmove2.
+            simpl.
+            rewrite !parmove_src_set. rewrite fst_combine; eauto with len.
+            eapply omap_var_defined_on; eauto.
+          }
+          pfold. eapply SimSilent.
+          * eapply plus2O. econstructor; eauto with len. reflexivity.
+          * eapply star2_plus2_plus2 with (A:=nil) (B:=nil); eauto.
+            eapply plus2O. econstructor; eauto. reflexivity. reflexivity.
+          * right; eapply (pmSim_sim p preg); try eapply LA1; eauto; simpl.
+            -- eapply (inRel_drop LA H4).
+            -- assert (getAnn al ⊆ blv) by eauto with cset.
+               eapply agree_on_incl.
+               symmetry. etransitivity.
+               eapply (@parmov_update_with_list (getAnn al));
+                 try rewrite eauto.
+               ++ rewrite snd_combine; eauto.
+               ++ assert (of_list Y' ⊆ lv). {
+                   eapply Ops.freeVars_live_list in H3.
+                   rewrite <- H3.
+                   rewrite of_list_freeVars_vars. reflexivity.
+                 }
+                 rewrite fst_combine, snd_combine; eauto.
+                 rewrite AL; eauto.
+               ++ rewrite fst_combine, snd_combine; eauto.
+                 rewrite disj_minus_eq; eauto.
+                 erewrite <- lookup_list_var_map; eauto.
+                 eapply update_with_list_agree; eauto with len.
+                 symmetry.
+                 eapply agree_on_incl; eauto. eauto with cset.
+                 rewrite H9. clear - H5. cset_tac.
+               ++ clear - H9 H5. cset_tac.
+            -- eapply defined_on_update_list; eauto with len.
+               assert (getAnn al \ of_list Z0 ⊆ lv). {
+                 rewrite <- H1. rewrite <- INCL. clear. cset_tac.
+               }
+               eauto using defined_on_incl.
+        - exploit (@list_to_stmt_correct
+                     ((proj1_sig lreg, lstmp)
+                        :: Parmov.parmove2 positive var_dec (fun _ : positive => pmtmp)
+                        (repl Y' (proj1_sig lreg) lstmp)
+                        (repl Z0 (proj1_sig lreg) lstmp) ++ (lstmp, proj1_sig lreg) :: nil)
+                     (stmtApp l nil) E' L'). {
+            unfold Parmov.parmove2.
+            simpl. rewrite moves_source_set_app; simpl.
+            rewrite !parmove_src_set. simpl. rewrite fst_combine; eauto with len.
+            edestruct (least_fresh_P_full_spec (part_1 p) (blv \ of_list Z0 ∪ lv)); dcr.
+            exploit (H10 (proj1_sig lreg)).
+            - subst lreg. destr_sig. eauto.
+            - subst lreg. destr_sig; dcr. simpl in *; dcr.
+              exploit (H12 (least_fresh_P (part_1 p) (blv \ of_list Z0 ∪ lv))); eauto.
+              + destruct H13; eauto. invc H13. subst reg.
+                set (reg:=least_fresh_P (part_1 p) (blv \ of_list Z0 ∪ lv)) in *.
+                exfalso. eapply NOTCOND.
+                eapply Pos.lt_eq_cases. eapply H12. eauto.
+            - rewrite of_list_repl_incl.
+              eapply defined_on_incl.
+              eapply defined_on_agree_eq; eauto.
+              eapply Ops.freeVars_live_list in H3.
+              rewrite <- of_list_freeVars_vars in H3. rewrite H3.
+              assert (IN:proj1_sig lreg ∈ lv). {
+                rewrite filter_incl in H9. rewrite H1 in H9.
+                clear - H9; cset_tac. eauto.
+              }
+              clear - IN. cset_tac.
+          }
+          pfold. eapply SimSilent.
+          * eapply plus2O. econstructor; eauto with len. reflexivity.
+          * eapply star2_plus2_plus2 with (A:=nil) (B:=nil); eauto.
+            eapply plus2O. econstructor; eauto. reflexivity. reflexivity.
+          * right; eapply pmSim_sim; try eapply LA1; eauto; simpl.
+            -- eapply (inRel_drop LA H4).
+            -- assert (getAnn al ⊆ blv) by eauto with cset.
+               symmetry. etransitivity. {
+                 eapply agree_on_incl.
+                 symmetry.
+                 eapply parmov_repl_agree; eauto.
+                 rewrite AL. eauto. rewrite AL; eauto.
+                 instantiate (1:=blv).
+                 rewrite H9. clear - H5 H6. cset_tac.
+               }
+               eapply agree_on_incl.
+               etransitivity.
+               eapply (@parmov_update_with_list (getAnn al));
+                 try rewrite eauto.
+               ++ rewrite snd_combine; eauto.
+               ++ assert (of_list Y' ⊆ lv). {
+                   eapply Ops.freeVars_live_list in H3.
+                   rewrite <- H3.
+                   rewrite of_list_freeVars_vars. reflexivity.
+                 }
+                 rewrite fst_combine, snd_combine; eauto.
+                 rewrite AL; eauto.
+               ++ rewrite fst_combine, snd_combine; eauto.
+                 rewrite disj_minus_eq; eauto.
+                 erewrite <- lookup_list_var_map; eauto.
+                 eapply update_with_list_agree; eauto with len.
+                 symmetry.
+                 eapply agree_on_incl; eauto. eauto with cset.
+                 rewrite H9. clear - H5. cset_tac.
+               ++ clear - H9 H5. cset_tac.
+            -- eapply defined_on_update_list; eauto with len.
+               assert (getAnn al \ of_list Z0 ⊆ lv). {
+                 rewrite <- H1. rewrite <- INCL. clear. cset_tac.
+               }
+               eauto using defined_on_incl.
+      }
     + perr.
   - pno_step. simpl. eauto using op_eval_live.
   - pone_step. right.
@@ -380,7 +690,7 @@ Proof.
     econstructor; eauto.
     + exploit H2; eauto.
     + eapply H2; eauto.
-    + simpl. reflexivity.
+    + eauto using defined_on_incl; eauto.
 Qed.
 
 End Implementation.
@@ -393,13 +703,13 @@ Proof.
     repeat let_pair_case_eq; eauto using noParams.
 Qed.
 
-Lemma pm_lower_noParams p ZL Lv s al
+Lemma pm_lower_noParams p ZL Lv s al preg
       (LS:live_sound Imperative ZL Lv s al)
-  : noParams (lower p (zip pair Lv ZL) s al).
+  : noParams (lower p preg (zip pair Lv ZL) s al).
 Proof.
   general induction LS; simpl;
     repeat let_pair_case_eq; repeat simpl_pair_eqs; subst; eauto using noParams.
-  - eauto using list_to_stmt_noParams, noParams.
+  - cases; eauto using list_to_stmt_noParams, noParams.
   - econstructor; intros; inv_get; simpl;
       try rewrite <- zip_app; eauto using noParams with len.
 Qed.
